sat.dfy
@@ -16,10 +16,10 @@ abstract module AbstractSatLib {
     function method cmp(f1: IntExpr, f2: IntExpr): BoolExpr
 
     function method {:verify false} sat(f1: BoolExpr): bool
+      ensures sat(getTrueBool())
 
       // Used for King Property 1
       //TODO: Possibly derive this from simpler rules
-      ensures sat(getTrueBool())
       ensures forall a,b :: sat(a) ==>
         sat(and(a,b)) || sat(and(a,not(b)))
 
@@ -28,11 +28,12 @@ abstract module AbstractSatLib {
       //ensures forall a,b,c,d ::
       //  sat(and( and(a, b), and(c, d) )) ==
       //  sat(and( and(a, c), and(b, d) ))
-      //ensures forall a,b ::
-      //  !sat(a) ==> !sat( and(a, b) )
-      //ensures forall a,b ::
-      //  sat( and(a, b) ) ==
-      //  sat( and(b, a) )
+      //ensures forall a,b,c :: sat( and(and(a,b),c) ) <==> sat( and(a,and(b,c)) )
+      ensures forall a,b ::
+        !sat(a) ==> !sat( and(a, b) )
+      ensures forall a,b ::
+        sat( and(a, b) ) ==
+        sat( and(b, a) )
 
 }
 
@@ -61,14 +62,14 @@ extern "NetworkSatLib" module NetworkSatLib {
         sat(and(a,b)) || sat(and(a,not(b)))
 
       // Used for King Property 2
-      //ensures forall a :: !sat(and(a, not(a)))
-      //ensures forall a,b,c,d ::
-      //  sat(and( and(a, b), and(c, d) )) ==
-      //  sat(and( and(a, c), and(b, d) ))
-      //ensures forall a,b ::
-      //  !sat(a) ==> !sat( and(a, b) )
-      //ensures forall a,b ::
-      //  sat( and(a, b) ) ==
-      //  sat( and(b, a) )
+      ensures forall a :: !sat(and(a, not(a)))
+      ensures forall a,b,c,d ::
+        sat(and( and(a, b), and(c, d) )) ==
+        sat(and( and(a, c), and(b, d) ))
+      ensures forall a,b ::
+        !sat(a) ==> !sat( and(a, b) )
+      ensures forall a,b ::
+        sat( and(a, b) ) ==
+        sat( and(b, a) )
 
 }
